

# Logical Foundations

Michał Stanisław Wójcik

December 26, 2025

## 1 Introduction

This document presents the logical foundations for a formal system based on first-order logic. The definitions and theorems presented here were designed by the human author. Claude AI assisted with writing proofs and definitions following the author's specifications and design. All AI-generated content in this paper has been carefully reviewed and verified by the human author.

## Contents

<b>1</b>	<b>Introduction</b>	<b>1</b>
<b>2</b>	<b>Well Formed Formula</b>	<b>2</b>
2.1	Syntax . . . . .	2
<b>3</b>	<b>Semantics</b>	<b>3</b>
<b>4</b>	<b>Substitutions</b>	<b>4</b>
4.1	Syntax . . . . .	4
4.2	Semantics . . . . .	6

## 2 Well Formed Formula

### 2.1 Syntax

Let  $\mathcal{V}$  be an infinite countable set of variable symbols. And  $\mathfrak{f}$  be a special predicate symbol.

**Definition 2.1.** Let  $\mathcal{P}$  be a set of predicate symbols for which  $\mathfrak{f} \in \mathcal{P}$  and  $\mathcal{F}$  be a set of function symbols. Let  $\mathfrak{a} : \mathcal{P} \cup \mathcal{F} \rightarrow \mathbb{N}$  be an arity function. then  $\mathcal{L} \stackrel{\text{def}}{=} (\mathcal{P}, \mathcal{F}, \mathfrak{a})$  is a signature of a language.

**Definition 2.2 (arity).** Let  $\mathcal{L} \stackrel{\text{def}}{=} (\mathcal{P}, \mathcal{F}, \mathfrak{a})$  be a signature of a language.

$$\mathcal{P}_k \stackrel{\text{def}}{=} \{p \in \mathcal{P} : \mathfrak{a}(p) = k\}, \quad (1)$$

$$\mathcal{F}_k \stackrel{\text{def}}{=} \{f \in \mathcal{F} : \mathfrak{a}(f) = k\}. \quad (2)$$

**Definition 2.3 (recursive: term).** Let  $\mathcal{L} = (\mathcal{P}, \mathcal{F}, \mathfrak{a})$  be a signature of a language.

1. For any  $v \in \mathcal{V}$ ,  $v$  is a **term**.
2. For any  $c \in \mathcal{F}_0$ ,  $c$  is a **term**.
3. For any  $f \in \mathcal{F}_k$  and  $\tau_1, \dots, \tau_k$  terms,  $f(\tau_1, \dots, \tau_k)$  is a **term**.

**Definition 2.4 (recursive: atomic formula).** Let  $\mathcal{L} = (\mathcal{P}, \mathcal{F}, \mathfrak{a})$  be a signature of a language.

1. For any  $p \in \mathcal{P}_0$ ,  $p$  is an **atomic formula**.
2. For any  $p \in \mathcal{P}_k$  and  $\tau_1, \dots, \tau_k$  are terms,  $p(\tau_1, \dots, \tau_k)$  is an **atomic formula**.

We will denote a set of all atomic formulas as  $\mathcal{A}(\mathcal{L})$ .

**Definition 2.5 (recursive: base formula, well formed formula).** Let  $\mathcal{L} = (\mathcal{P}, \mathcal{F}, \mathfrak{a})$  be a signature of a language.

1. For any atomic formula  $\phi$ ,  $\phi$  is a **base formula**.
2. For any **base formula**  $\phi$ ,  $\phi$  is a **well formed formula**.
3. For any **well formed formula**  $\phi$ ,  $(\phi)$  is a **base formula**.
4. For any **base formulas**  $\alpha, \beta$ ,  $\alpha \rightarrow \beta$  is a **well formed formula**.
5. For any  $v \in \mathcal{V}$  and a **base formula**  $\phi$ ,  $\forall v. \phi$  is a **well formed formula**.

We will denote set of all base formulas as  $\mathcal{B}(\mathcal{L})$  and set of all well formed formulas as  $\mathcal{F}(\mathcal{L})$ .

**Note 2.6 (syntactic equality).** We use the notation  $\stackrel{\text{sx}}{=}$  to denote syntactic equality of terms and formulas. Two terms (or formulas) are syntactically equal if they are the same syntactic construct.

### 3 Semantics

**Definition 3.1** ( $\mathcal{L}$ -structure). Let  $\mathcal{L} = (\mathcal{P}, \mathcal{F}, \mathbf{a})$  be a signature of a language and  $A$  be an arbitrary mathematical domain, then a mapping  $\mathbf{M}$  such that

$$\mathbf{M} : \mathcal{P} \cup \mathcal{F} \rightarrow \{0, 1\} \cup \bigcup_{k=1}^{\infty} \{0, 1\}^{(A^k)} \cup A \cup \bigcup_{k=1}^{\infty} A^{(A^k)}, \quad (3)$$

where  $\mathbf{M}(\mathbf{f}) = 0$ ,

$$\mathbf{M}(\mathcal{P}_0) \subset \{0, 1\} \text{ and } \mathbf{M}(\mathcal{P}_k) \subset \{0, 1\}^{(A^k)} \text{ for } k = 1, \dots, \quad (4)$$

and

$$\mathbf{M}(\mathcal{F}_0) \subset A \text{ and } \mathbf{M}(\mathcal{F}_k) \subset A^{(A^k)} \text{ for } k = 1, \dots \quad (5)$$

is called an  $\mathcal{L}$ -structure with domain  $A$ .

For convenience we will denote values of  $\mathbf{M}$  as  $p^{\mathbf{M}} \stackrel{\text{def}}{=} \mathbf{M}(p)$  for  $p \in \mathcal{P}$  and  $f^{\mathbf{M}} \stackrel{\text{def}}{=} \mathbf{M}(f)$  for  $f \in \mathcal{F}$ .

**Definition 3.2** (assignment). Let  $A$  be an arbitrary mathematical domain. Then  $j : \mathcal{V} \rightarrow A$  is called an variables assignment in  $A$ .

**Definition 3.3** (recursive: term evaluation). Let  $\mathcal{L} = (\mathcal{P}, \mathcal{F}, \mathbf{a})$  be a signature of a language and  $A$  be an arbitrary mathematical domain, let  $\mathbf{M}$  be an  $\mathcal{L}$ -structure and  $j : \mathcal{V} \rightarrow A$ . Let  $\tau$  be an arbitrary term.

1. If  $\tau \stackrel{\text{sx}}{=} v$  where  $v \in \mathcal{V}$ , then  $\tau^{\mathbf{M}, j} \stackrel{\text{def}}{=} j(v)$ .
2. If  $\tau \stackrel{\text{sx}}{=} f$  where  $f \in \mathcal{F}_0$ , then  $\tau^{\mathbf{M}, j} \stackrel{\text{def}}{=} f^{\mathbf{M}}$ .
3. If  $\tau \stackrel{\text{sx}}{=} f(\tau_1, \dots, \tau_k)$  where  $f \in \mathcal{F}_k$  and  $\tau_1, \dots, \tau_k$  are terms, then  $\tau^{\mathbf{M}, j} \stackrel{\text{def}}{=} f^{\mathbf{M}}(\tau_1^{\mathbf{M}, j}, \dots, \tau_k^{\mathbf{M}, j})$ .

**Definition 3.4.** Let  $\mathcal{L}$  be a signature of a language. Let  $\mathbf{M}$  be a  $\mathcal{L}$ -structure with domain  $A$  and let  $j : \mathcal{V} \rightarrow A$  be an assignment of variables. Then we define

$$j \frac{a}{x}(v) \stackrel{\text{def}}{=} \begin{cases} a & \text{if } v \text{ is } x, \\ j(v) & \text{otherwise.} \end{cases} \quad (6)$$

For the purposes of this work, we will define product of infinite number of 0s and 1s.

**Definition 3.5.** Let  $S$  be an arbitrary set and  $a_s \in \{0, 1\}$  for any  $s \in S$ .

$$\prod_{s \in S} a_s = \begin{cases} 1 & \text{if } a_s = 1 \text{ for all } s \in S, \\ 0 & \text{otherwise.} \end{cases} \quad (7)$$

**Definition 3.6 (recursive: formula evaluation).** Let  $\mathcal{L} = (\mathcal{P}, \mathcal{F}, \mathbf{a})$  be a signature of a language and  $A$  be an arbitrary mathematical domain, let  $\mathbf{M}$  be an  $\mathcal{L}$ -structure with domain  $A$  and  $j : \mathcal{V} \rightarrow A$ . Let  $\phi \in \mathcal{F}(\mathcal{L})$ .

1. If  $\phi \equiv^{\text{sx}} p$  where  $p \in \mathcal{P}$ , then  $\phi^{\mathbf{M},j} \stackrel{\text{def}}{=} p^{\mathbf{M}}$ .
2. If  $\phi \equiv^{\text{sx}} p(\tau_1, \dots, \tau_k)$  where  $p \in \mathcal{P}_k$  and  $\tau_1, \dots, \tau_k$  are terms, then  $\phi^{\mathbf{M},j} \stackrel{\text{def}}{=} p^{\mathbf{M}}(\tau_1^{\mathbf{M},j}, \dots, \tau_k^{\mathbf{M},j})$ .
3. If  $\phi \equiv^{\text{sx}} \alpha \rightarrow \beta$  where  $\alpha, \beta \in \mathcal{B}(\mathcal{L})$ , then

$$\phi^{\mathbf{M},j} \stackrel{\text{def}}{=} 1 - \alpha^{\mathbf{M},j}(1 - \beta^{\mathbf{M},j}). \quad (8)$$

4. If  $\phi \equiv^{\text{sx}} \forall x. \psi$  where  $x \in \mathcal{V}$  and  $\psi \in \mathcal{B}(\mathcal{L})$ , then

$$\phi^{\mathbf{M},j} \stackrel{\text{def}}{=} \prod_{a \in A} \psi^{\mathbf{M},j} \frac{a}{x}. \quad (9)$$

**Corollary 3.7.** Let  $\mathcal{L} = (\mathcal{P}, \mathcal{F}, \mathbf{a})$  be a signature of a language and  $A$  be an arbitrary mathematical domain, let  $\mathbf{M}$  be an  $\mathcal{L}$ -structure with domain  $A$  and  $j : \mathcal{V} \rightarrow A$ . Let  $\phi \in \mathcal{F}(\mathcal{L})$ , then

$$(\phi \rightarrow \mathbf{f})^{\mathbf{M},j} = 1 - \phi^{\mathbf{M},j}. \quad (10)$$

**Definition 3.8 (model).** Let  $\mathcal{L} = (\mathcal{P}, \mathcal{F}, \mathbf{a})$  be a signature of a language and  $A$  be an arbitrary mathematical domain, let  $\mathbf{M}$  be an  $\mathcal{L}$ -structure with domain  $A$  and  $j : \mathcal{V} \rightarrow A$ . Let  $\phi \in \mathcal{F}(\mathcal{L})$ , then

$$\mathbf{M}, j \models \phi \stackrel{\text{def}}{\iff} \phi^{\mathbf{M},j} = 1. \quad (11)$$

## 4 Substitutions

### 4.1 Syntax

**Definition 4.1 (recursive: variable in a term).** Let  $\mathcal{L} = (\mathcal{P}, \mathcal{F}, \mathbf{a})$  be a signature of a language. Let  $v \in \mathcal{V}$  and  $\tau$  be a term.

1. If  $\tau \equiv^{\text{sx}} v$  then  $v$  is a **variable in** term  $\tau$ .
2. If  $\tau \equiv^{\text{sx}} f(\tau_1, \dots, \tau_k)$  where  $f \in \mathcal{F}_k$  and  $\tau_1, \dots, \tau_k$  are terms and  $v$  is a **variable in** some term  $\tau_i$  where  $i$  is an integer with  $1 \leq i \leq k$ , then  $v$  is a **variable in** term  $\tau$ .
3. Otherwise  $v$  is not a **variable in** a term  $\tau$ .

**Definition 4.2 (recursive: variable in a well formed formula).** Let  $\mathcal{L} = (\mathcal{P}, \mathcal{F}, \mathbf{a})$  be a signature of a language. Let  $v \in \mathcal{V}$  and  $\phi \in \mathcal{F}(\mathcal{L})$ .

1. If  $\phi \stackrel{\text{sx}}{=} p(\tau_1, \dots, \tau_k)$  where  $p \in \mathcal{P}_k$  and  $\tau_1, \dots, \tau_k$  are terms, and  $v$  is a **variable in** some term  $\tau_i$  where  $i$  is an integer with  $1 \leq i \leq k$ , then  $v$  is a **variable in**  $\phi$ .
2. If  $\phi \stackrel{\text{sx}}{=} \alpha \rightarrow \beta$  where  $\alpha, \beta \in \mathcal{B}(\mathcal{L})$ , and  $v$  is a **variable in**  $\alpha$  or  $v$  is a **variable in**  $\beta$ , then  $v$  is a **variable in**  $\phi$ .
3. If  $\phi \stackrel{\text{sx}}{=} \forall x. \psi$  where  $x \in \mathcal{V}$  and  $\psi \in \mathcal{B}(\mathcal{L})$ , and either  $v = x$  or  $v$  is a **variable in**  $\psi$ , then  $v$  is a **variable in**  $\phi$ .
4. Otherwise  $v$  is not a **variable in**  $\phi$ .

**Definition 4.3 (recursive: free variable in a well formed formula).** Let  $\mathcal{L} = (\mathcal{P}, \mathcal{F}, \mathbf{a})$  be a signature of a language. Let  $v \in \mathcal{V}$  and  $\phi \in \mathcal{F}(\mathcal{L})$ .

1. If  $\phi \in \mathcal{A}(\mathcal{L})$  and  $v$  is a variable in  $\phi$ , then  $v$  is a **free variable in**  $\phi$ .
2. If  $\phi \stackrel{\text{sx}}{=} \alpha \rightarrow \beta$  where  $\alpha, \beta \in \mathcal{B}(\mathcal{L})$ , and  $v$  is a **free variable in**  $\alpha$  or  $v$  is a **free variable in**  $\beta$ , then  $v$  is a **free variable in**  $\phi$ .
3. If  $\phi \stackrel{\text{sx}}{=} \forall x. \psi$  where  $x \in \mathcal{V}$  and  $\psi \in \mathcal{B}(\mathcal{L})$  and  $v$  is not  $x$  and  $v$  is a **free variable in**  $\psi$ , then  $v$  is a **free variable in**  $\phi$ .
4. Otherwise  $v$  is not a **free variable in**  $\phi$ .

**Definition 4.4 (recursive: substitution in term).** Let  $\mathcal{L} = (\mathcal{P}, \mathcal{F}, \mathbf{a})$  be a signature of a language. Let  $x \in \mathcal{V}$  and  $\tau, \sigma$  be terms.

1. If  $\sigma \stackrel{\text{sx}}{=} x$ , then  $\sigma(x/\tau) \stackrel{\text{def}}{=} \tau$ .
2. If  $\sigma \stackrel{\text{sx}}{=} v$  where  $v \in \mathcal{V}$  and  $v$  is not  $x$ , then  $\sigma(x/\tau) \stackrel{\text{def}}{=} v$ .
3. If  $\sigma \stackrel{\text{sx}}{=} c$  where  $c \in \mathcal{F}_0$ , then  $\sigma(x/\tau) \stackrel{\text{def}}{=} c$ .
4. If  $\sigma \stackrel{\text{sx}}{=} f(\sigma_1, \dots, \sigma_k)$  where  $f \in \mathcal{F}_k$  and  $\sigma_1, \dots, \sigma_k$  are terms, then  $\sigma(x/\tau) \stackrel{\text{def}}{=} f(\sigma_1(x/\tau), \dots, \sigma_k(x/\tau))$ .

**Definition 4.5 (recursive: substitution in well formed formula).** Let  $\mathcal{L} = (\mathcal{P}, \mathcal{F}, \mathbf{a})$  be a signature of a language. Let  $x \in \mathcal{V}$ ,  $\tau$  be a term, and  $\phi \in \mathcal{F}(\mathcal{L})$ .

1. If  $\phi \stackrel{\text{sx}}{=} p$  where  $p \in \mathcal{P}_0$ , then  $\phi(x/\tau) \stackrel{\text{def}}{=} p$ .
2. If  $\phi \stackrel{\text{sx}}{=} p(\sigma_1, \dots, \sigma_k)$  where  $p \in \mathcal{P}_k$  and  $\sigma_1, \dots, \sigma_k$  are terms, then  $\phi(x/\tau) \stackrel{\text{def}}{=} p(\sigma_1(x/\tau), \dots, \sigma_k(x/\tau))$ .
3. If  $\phi \stackrel{\text{sx}}{=} \alpha \rightarrow \beta$  where  $\alpha, \beta \in \mathcal{B}(\mathcal{L})$ , then  $\phi(x/\tau) \stackrel{\text{def}}{=} \alpha(x/\tau) \rightarrow \beta(x/\tau)$ .
4. If  $\phi \stackrel{\text{sx}}{=} \forall y. \psi$  where  $y \in \mathcal{V}$  and  $\psi \in \mathcal{B}(\mathcal{L})$  and  $y \stackrel{\text{sx}}{=} x$ , then  $\phi(x/\tau) \stackrel{\text{def}}{=} \forall y. \psi$ .

5. If  $\phi \stackrel{\text{sx}}{=} \forall y. \psi$  where  $y \in \mathcal{V}$  and  $\psi \in \mathcal{B}(\mathcal{L})$  and  $y$  is not  $x$  and  $y$  is not a variable in  $\tau$ , then  $\phi(x/\tau) \stackrel{\text{def}}{=} \forall y. \psi(x/\tau)$ .
6. Otherwise  $\phi(x/\tau)$  is **not admissible**.

**Lemma 4.6.** Let  $\mathcal{L} = (\mathcal{P}, \mathcal{F}, \mathbf{a})$  be a signature of a language. Let  $\sigma$  be a term. Let  $x \in \mathcal{V}$  and  $\tau$  be a term. Let  $y \in \mathcal{V}$  and  $y$  is not in term  $\tau$  and  $y$  is not in term  $\sigma$ . Then

$$\sigma(x/y)(y/\tau) \stackrel{\text{sx}}{=} \sigma(x/\tau). \quad (12)$$

*Proof.* We proceed by structural induction on the term  $\sigma$ .

**Case 1:**  $\sigma \stackrel{\text{sx}}{=} x$ .

Then  $\sigma(x/y) \stackrel{\text{sx}}{=} y$ , and

$$(\sigma(x/y))(y/\tau) \stackrel{\text{sx}}{=} y(y/\tau) \stackrel{\text{sx}}{=} \tau.$$

Also,  $\sigma(x/\tau) \stackrel{\text{sx}}{=} \tau$ . Therefore,  $\sigma(x/y)(y/\tau) \stackrel{\text{sx}}{=} \sigma(x/\tau)$ .

**Case 2:**  $\sigma \stackrel{\text{sx}}{=} v$  where  $v \in \mathcal{V}$  and  $v \neq x$ .

Since  $y$  is not a **variable in**  $\sigma$ , we have  $v \neq y$ . Then  $\sigma(x/y) \stackrel{\text{sx}}{=} v$ , and

$$(\sigma(x/y))(y/\tau) \stackrel{\text{sx}}{=} v(y/\tau) \stackrel{\text{sx}}{=} v$$

(since  $v \neq y$ ). Also,  $\sigma(x/\tau) \stackrel{\text{sx}}{=} v$  (since  $v \neq x$ ). Therefore,  $\sigma(x/y)(y/\tau) \stackrel{\text{sx}}{=} \sigma(x/\tau)$ .

**Case 3:**  $\sigma \stackrel{\text{sx}}{=} c$  where  $c \in \mathcal{F}_0$ .

Then  $\sigma(x/y) \stackrel{\text{sx}}{=} c$ , and

$$(\sigma(x/y))(y/\tau) \stackrel{\text{sx}}{=} c(y/\tau) \stackrel{\text{sx}}{=} c.$$

Also,  $\sigma(x/\tau) \stackrel{\text{sx}}{=} c$ . Therefore,  $\sigma(x/y)(y/\tau) \stackrel{\text{sx}}{=} \sigma(x/\tau)$ .

**Case 4:**  $\sigma \stackrel{\text{sx}}{=} f(\sigma_1, \dots, \sigma_k)$  where  $f \in \mathcal{F}_k$  and  $\sigma_1, \dots, \sigma_k$  are terms.

Since  $y$  is not a **variable in**  $\sigma$ ,  $y$  is not a **variable in** any  $\sigma_i$  for  $i = 1, \dots, k$ . By the definition of substitution in term,  $\sigma(x/y) \stackrel{\text{sx}}{=} f(\sigma_1(x/y), \dots, \sigma_k(x/y))$ . Then

$$(\sigma(x/y))(y/\tau) \stackrel{\text{sx}}{=} f(\sigma_1(x/y)(y/\tau), \dots, \sigma_k(x/y)(y/\tau)).$$

By inductive hypothesis,  $\sigma_i(x/y)(y/\tau) \stackrel{\text{sx}}{=} \sigma_i(x/\tau)$  for all  $i = 1, \dots, k$ . Therefore,

$$(\sigma(x/y))(y/\tau) \stackrel{\text{sx}}{=} f(\sigma_1(x/\tau), \dots, \sigma_k(x/\tau)) \stackrel{\text{sx}}{=} \sigma(x/\tau).$$

This completes the proof by structural induction.  $\square$

## 4.2 Semantics

**Lemma 4.7.** Let  $\mathcal{L}$  be a signature of a language and  $A$  be an arbitrary mathematical domain. Let  $\mathbf{M}$  be an  $\mathcal{L}$ -structure with domain  $A$  and  $j : \mathcal{V} \rightarrow A$  be an assignment. For any term  $\sigma$ , any  $x \in \mathcal{V}$ , and any term  $\tau$ , we have

$$\sigma \stackrel{\mathbf{M}, j}{\tau} \frac{\tau^{(\mathbf{M}, j)}}{x} = (\sigma(x/\tau))^{\mathbf{M}, j}. \quad (13)$$

*Proof.* We proceed by structural induction on the term  $\sigma$ .

**Case 1:**  $\sigma \stackrel{\text{sx}}{=} x$ .

Then  $\sigma(x/\tau) \stackrel{\text{sx}}{=} \tau$  and

$$\sigma^{\mathbf{M},j} \frac{\tau^{(\mathbf{M},j)}}{x} = (j \frac{\tau^{(\mathbf{M},j)}}{x})(x) = \tau^{\mathbf{M},j} = (\sigma(x/\tau))^{\mathbf{M},j}.$$

**Case 2:**  $\sigma \stackrel{\text{sx}}{=} v$  where  $v \in \mathcal{V}$  and  $v \neq x$ .

Then  $\sigma(x/\tau) \stackrel{\text{sx}}{=} v$  and

$$\sigma^{\mathbf{M},j} \frac{\tau^{(\mathbf{M},j)}}{x} = (j \frac{\tau^{(\mathbf{M},j)}}{x})(v) = j(v) = v^{\mathbf{M},j} = (\sigma(x/\tau))^{\mathbf{M},j}.$$

**Case 3:**  $\sigma \stackrel{\text{sx}}{=} c$  where  $c \in \mathcal{F}_0$ .

Then  $\sigma(x/\tau) \stackrel{\text{sx}}{=} c$  and

$$\sigma^{\mathbf{M},j} \frac{\tau^{(\mathbf{M},j)}}{x} = c^{\mathbf{M}} = (\sigma(x/\tau))^{\mathbf{M},j}.$$

**Case 4:**  $\sigma \stackrel{\text{sx}}{=} f(\sigma_1, \dots, \sigma_k)$  where  $f \in \mathcal{F}_k$  and  $\sigma_1, \dots, \sigma_k$  are terms.

Then  $\sigma(x/\tau) \stackrel{\text{sx}}{=} f(\sigma_1(x/\tau), \dots, \sigma_k(x/\tau))$ . By inductive hypothesis,  $\sigma_i^{\mathbf{M},j} \frac{\tau^{(\mathbf{M},j)}}{x} = (\sigma_i(x/\tau))^{\mathbf{M},j}$  for all  $i = 1, \dots, k$ . Thus

$$\begin{aligned} \sigma^{\mathbf{M},j} \frac{\tau^{(\mathbf{M},j)}}{x} &= f^{\mathbf{M}}(\sigma_1^{\mathbf{M},j} \frac{\tau^{(\mathbf{M},j)}}{x}, \dots, \sigma_k^{\mathbf{M},j} \frac{\tau^{(\mathbf{M},j)}}{x}) \\ &= f^{\mathbf{M}}((\sigma_1(x/\tau))^{\mathbf{M},j}, \dots, (\sigma_k(x/\tau))^{\mathbf{M},j}) \\ &= (f(\sigma_1(x/\tau), \dots, \sigma_k(x/\tau)))^{\mathbf{M},j} \\ &= (\sigma(x/\tau))^{\mathbf{M},j}. \end{aligned}$$

This completes the proof by structural induction.  $\square$

**Theorem 4.8.** Let  $\mathcal{L}$  be a signature of a language. Let  $\phi \in \mathcal{F}(\mathcal{L})$  and let  $\tau$  be an arbitrary term. If  $\phi(x/\tau)$  is admissible, then for any  $\mathcal{L}$ -structure  $\mathbf{M}$  with domain  $A$  and for any assignment of variables  $j : \mathcal{V} \rightarrow A$  we have

$$(\mathbf{M}, j \frac{\tau^{(\mathbf{M},j)}}{x}) \models \phi \iff (\mathbf{M}, j) \models \phi(x/\tau). \quad (14)$$

*Proof.* We proceed by structural induction on  $\phi \in \mathcal{F}(\mathcal{L})$ .

**Case 1:**  $\phi \stackrel{\text{sx}}{=} p$  where  $p \in \mathcal{P}_0$ .

By the definition of substitution in well formed formula,  $\phi(x/\tau) \stackrel{\text{sx}}{=} p$ . By the definition of formula evaluation,  $\phi^{\mathbf{M},j} = p^{\mathbf{M}}$  for any assignment  $j$ . Thus

$$\begin{aligned}
(\mathbf{M}, j \frac{\tau(\mathbf{M},j)}{x}) \models \phi &\iff \phi^{\mathbf{M},j \frac{\tau(\mathbf{M},j)}{x}} = 1 \\
&\iff p^{\mathbf{M}} = 1 \\
&\iff \phi^{\mathbf{M},j} = 1 \\
&\iff (\mathbf{M}, j) \models \phi \\
&\iff (\mathbf{M}, j) \models \phi(x/\tau).
\end{aligned}$$

**Case 2:**  $\phi \stackrel{\text{sx}}{=} p(\sigma_1, \dots, \sigma_k)$  where  $p \in \mathcal{P}_k$  and  $\sigma_1, \dots, \sigma_k$  are terms.

By the definition of substitution in well formed formula,  $\phi(x/\tau) \stackrel{\text{sx}}{=} p(\sigma_1(x/\tau), \dots, \sigma_k(x/\tau))$ .

By Lemma 4.7, for each term  $\sigma_i$ , we have  $\sigma_i^{\mathbf{M},j \frac{\tau(\mathbf{M},j)}{x}} = (\sigma_i(x/\tau))^{\mathbf{M},j}$ . Therefore,

$$\begin{aligned}
(\mathbf{M}, j \frac{\tau(\mathbf{M},j)}{x}) \models \phi &\iff \phi^{\mathbf{M},j \frac{\tau(\mathbf{M},j)}{x}} = 1 \\
&\iff p^{\mathbf{M}}(\sigma_1^{\mathbf{M},j \frac{\tau(\mathbf{M},j)}{x}}, \dots, \sigma_k^{\mathbf{M},j \frac{\tau(\mathbf{M},j)}{x}}) = 1 \\
&\iff p^{\mathbf{M}}((\sigma_1(x/\tau))^{\mathbf{M},j}, \dots, (\sigma_k(x/\tau))^{\mathbf{M},j}) = 1 \\
&\iff (p(\sigma_1(x/\tau), \dots, \sigma_k(x/\tau)))^{\mathbf{M},j} = 1 \\
&\iff (\phi(x/\tau))^{\mathbf{M},j} = 1 \\
&\iff (\mathbf{M}, j) \models \phi(x/\tau).
\end{aligned}$$

**Case 3:**  $\phi \stackrel{\text{sx}}{=} \alpha \rightarrow \beta$  where  $\alpha, \beta \in \mathcal{B}(\mathcal{L})$ .

By the definition of substitution in well formed formula,  $\phi(x/\tau) \stackrel{\text{sx}}{=} \alpha(x/\tau) \rightarrow \beta(x/\tau)$ . By inductive hypothesis,

$$\begin{aligned}
(\mathbf{M}, j \frac{\tau(\mathbf{M},j)}{x}) \models \alpha &\iff (\mathbf{M}, j) \models \alpha(x/\tau), \\
(\mathbf{M}, j \frac{\tau(\mathbf{M},j)}{x}) \models \beta &\iff (\mathbf{M}, j) \models \beta(x/\tau).
\end{aligned}$$



By the definition of formula evaluation,

$$\begin{aligned}
(\mathbf{M}, j \frac{\tau(\mathbf{M}, j)}{x}) \models \phi &\iff \phi^{\mathbf{M}, j \frac{\tau(\mathbf{M}, j)}{x}} = 1 \\
&\iff 1 - \alpha^{\mathbf{M}, j \frac{\tau(\mathbf{M}, j)}{x}} (1 - \beta^{\mathbf{M}, j \frac{\tau(\mathbf{M}, j)}{x}}) = 1 \\
&\iff 1 - (\alpha(x/\tau))^{\mathbf{M}, j} (1 - (\beta(x/\tau))^{\mathbf{M}, j}) = 1 \\
&\iff (\alpha(x/\tau) \rightarrow \beta(x/\tau))^{\mathbf{M}, j} = 1 \\
&\iff (\phi(x/\tau))^{\mathbf{M}, j} = 1 \\
&\iff (\mathbf{M}, j) \models \phi(x/\tau).
\end{aligned}$$

**Case 4:**  $\phi \stackrel{\text{sx}}{=} \forall y. \psi$  where  $y \in \mathcal{V}$  and  $\psi \in \mathcal{B}(\mathcal{L})$ .

**Subcase 4a:** If  $y = x$ , then by the definition of substitution,  $\phi(x/\tau) \stackrel{\text{sx}}{=} \forall y. \psi$ . Thus

$$\begin{aligned}
(\mathbf{M}, j \frac{\tau(\mathbf{M}, j)}{x}) \models \phi &\iff \phi^{\mathbf{M}, j \frac{\tau(\mathbf{M}, j)}{x}} = 1 \\
&\iff \prod_{a \in A} \psi^{\mathbf{M}, (j \frac{\tau(\mathbf{M}, j)}{x}) \frac{a}{y}} = 1 \\
&\iff \prod_{a \in A} \psi^{\mathbf{M}, j \frac{a}{y}} = 1 \quad (\text{since } y = x \text{ and } (j \frac{\tau(\mathbf{M}, j)}{x}) \frac{a}{x} = j \frac{a}{x}) \\
&\iff \phi^{\mathbf{M}, j} = 1 \\
&\iff (\mathbf{M}, j) \models \phi \\
&\iff (\mathbf{M}, j) \models \phi(x/\tau).
\end{aligned}$$

**Subcase 4b:** If  $y \neq x$  and  $y$  is not a **variable in**  $\tau$ , then by the definition of substitution,  $\phi(x/\tau) \stackrel{\text{sx}}{=} \forall y. \psi(x/\tau)$ . By inductive hypothesis, for any  $a \in A$ ,

$$(\mathbf{M}, j \frac{a \tau^{\mathbf{M}, j \frac{a}{y}}}{x}) \models \psi \iff (\mathbf{M}, j \frac{a}{y}) \models \psi(x/\tau).$$

Since  $y$  is not a **variable in**  $\tau$ , the evaluation of  $\tau$  does not depend on the value

assigned to  $y$ . Therefore,  $\tau^{\mathbf{M}, j \frac{a}{y}} = \tau^{\mathbf{M}, j}$  for all  $a \in A$ .

Moreover, since  $x \neq y$ , we have  $j \frac{\tau^{\mathbf{M}, j} a}{x} \frac{a}{y} = j \frac{a \tau^{\mathbf{M}, j}}{y} \frac{a}{x}$  for all  $a \in A$ .

Thus,

$$\begin{aligned}
(\mathbf{M}, j \frac{\tau(\mathbf{M}, j)}{x}) \models \phi &\iff \phi^{\mathbf{M}, j \frac{\tau(\mathbf{M}, j)}{x}} = 1 \\
&\iff \prod_{a \in A} \psi^{\mathbf{M}, (j \frac{\tau(\mathbf{M}, j)}{x}) \frac{a}{y}} = 1 \\
&\iff \prod_{a \in A} \psi^{\mathbf{M}, j \frac{a \tau(\mathbf{M}, j)}{y x}} = 1 \\
&\iff \prod_{a \in A} (\psi(x/\tau))^{\mathbf{M}, j \frac{a}{y}} = 1 \quad (\text{by inductive hypothesis}) \\
&\iff (\forall y. \psi(x/\tau))^{\mathbf{M}, j} = 1 \\
&\iff (\phi(x/\tau))^{\mathbf{M}, j} = 1 \\
&\iff (\mathbf{M}, j) \models \phi(x/\tau).
\end{aligned}$$

This completes the proof by structural induction. □